examples/stp_test.v
@@ -1,5 +1,5 @@
 Require Import isla.isla.
-Require Import isla.instructions.stp.
+Require Import isla.instructions.instr_stp.
 
 Definition spec `{!islaG Σ} `{!threadG} a sp (v1 v2 : bv 64) : iProp Σ :=
   ∃ (vold1 vold2 : bv 64),
@@ -20,7 +20,7 @@ Definition spec `{!islaG Σ} `{!threadG} a sp (v1 v2 : bv 64) : iProp Σ :=
     True).
 
 Lemma stp_wp `{!islaG Σ} `{!threadG} (sp v1 v2: bv 64):
-  instr 0x0000000010300000 (Some aa9bf07e0) -∗
+  instr 0x0000000010300000 (Some instr_stp) -∗
   instr_body 0x0000000010300000 (spec 0x0000000010300004 sp v1 v2).
 Proof.
   iStartProof.
